Clean/Test.lean
@@ -26,6 +26,7 @@ import Clean.Halo2.Tests.TestVkMatchFullWidth
 import Clean.Halo2.Tests.TestVkMatchShort
 import Clean.Halo2.Tests.TestVkMatchAction
 import Clean.Halo2.Tests.TestVkLayoutAction
+import Clean.Halo2.Tests.TestVkLayoutActionBase
 import Clean.Halo2.Tests.TestVkMatchSinsemilla
 import Clean.Halo2.Tests.TestVkMatchMerkle
 import Clean.Halo2.Tests.TestVkLayoutMul
